src/riscv/Platform/LogInstructionTrace.v
@@ -1,0 +1,76 @@
+Require Import Coq.ZArith.ZArith.
+Require Import Coq.Lists.List.
+Require Import riscv.Utility.Monads. Import StateAbortFailOperations.
+Require Import riscv.Utility.MonadNotations.
+Require Import riscv.Spec.Decode.
+Require Import riscv.Spec.Machine.
+Require Import riscv.Utility.Utility.
+Require Import riscv.Spec.Primitives.
+Require Import riscv.Utility.ExtensibleRecords.
+Require Import coqutil.Z.Lia.
+Require Import coqutil.Map.Interface.
+
+Local Open Scope Z_scope.
+Local Open Scope bool_scope.
+Import ListNotations.
+
+Definition pc: nat := 1.
+Definition mem: nat := 3.
+Definition exectrace: nat := 8.
+
+Definition ExecTrace: Type := list (Z * Instruction). (* pc and instruction *)
+
+Section Riscv.
+  Context {W: Words}.
+  Context {Mem: map.map word byte}.
+  Context (UnknownFields: natmap Type).
+
+  Definition Fields: natmap Type := natmap.putmany UnknownFields [
+    (pc, word: Type);
+    (mem, Mem: Type);
+    (exectrace, ExecTrace)
+   ].
+
+  Definition State: Type := hnatmap Fields.
+
+  Import HnatmapNotations. Open Scope hnatmap_scope.
+
+  Local Notation get := (@StateAbortFailOperations.get State). (* to improve type inference *)
+
+  Global Instance AddExecTrace(RVP: RiscvProgram (StateAbortFail State) word):
+    RiscvProgram (StateAbortFail State) word := {
+    getRegister := getRegister;
+    setRegister := setRegister;
+    getPC := getPC;
+    setPC := setPC;
+    loadByte := loadByte;
+    loadHalf := loadHalf;
+    loadWord kind addr :=
+      v <- loadWord kind addr;
+      match kind with
+      | Fetch => mach <- get;
+                 let i := match Memory.loadWord mach[mem] mach[pc] with
+                          | Some i => LittleEndian.combine 4 i
+                          | None => -1
+                          end in
+                 put mach[exectrace := (word.unsigned mach[pc], decode RV64IMAF i) :: mach[exectrace]];;
+                 Return v
+      | _ => Return v
+      end;
+    loadDouble := loadDouble;
+    storeByte := storeByte;
+    storeHalf := storeHalf;
+    storeWord := storeWord;
+    storeDouble := storeDouble;
+    makeReservation := makeReservation;
+    clearReservation := clearReservation;
+    checkReservation := checkReservation;
+    getCSRField := getCSRField;
+    setCSRField := setCSRField;
+    getPrivMode := getPrivMode;
+    setPrivMode := setPrivMode;
+    endCycleNormal := endCycleNormal;
+    endCycleEarly{A} := @endCycleEarly _ _ _ _ _ A;
+  }.
+
+End Riscv.
